밀러 라빈 알고리즘 사용

$$a^{2^kq} \equiv 1$$

$$a^{2^kq} - 1 \equiv 0$$
$$=(a^{2^{k-1}q} + 1)(a^{2^{k-2}q} + 1)\cdots (a^q + 1)(a^q - 1) = 0$$
~~~c
int miller_rabin(uint64_t n) {
	if (n == 1) return COMPOSITE;
	if (n <= 3) return PRIME;
	if (n % 2 == 0) return COMPOSITE;
	uint64_t d = n - 1;
	int r = 0;
	while (d % 2 == 0) {
		d /= 2;
		r++;
	}
	for (int i = 0; i < BASELEN; i++) {
		if (a[i] % n == 0) return PRIME;
			uint64_t x = mod_pow(a[i], d, n);
		if (x == 1 || x == n - 1) {
			continue;
		}
		for (int j = 0; j < r - 1; j++) {
			x = mod_pow(x, 2, n);
			if (x == n - 1) {
				break;
			}
		}
		if (x != n - 1) {
			return COMPOSITE; // 소수가 아님
		}
	}
	return PRIME;
}
~~~
